rocq-brick-libstdcpp/test/g4g_trace/endl_spec_test.v
@@ -1,0 +1,10 @@
+(**
+ * Copyright (c) 2026 SkyLabs AI, Inc.
+ * This software is distributed under the terms of the BedRock Open-Source License.
+ * See the LICENSE-BedRock file in the repository root for details.
+ *)
+Require Import skylabs.auto.cpp.specs.
+Require Import skylabs.brick.libstdcpp.iostream_trace.spec.
+
+Example endl_content_is_line_feed :
+  BS.string_to_bytes endl_content = [10%N] := eq_refl.
