rocq-brick-libstdcpp/test/g4g_trace/N12_area.v
@@ -18,7 +18,7 @@ Section with_cpp.
     \pre{str} _global "std::cout" |-> ostream_contentR 1$m str
     \post[Vint 0]
       _global "std::cout" |-> ostream_contentR 1$m
-        (str ++ "Area = " ++ Z_to_string (area_of_rectangle side1 side2) ++ "\n" ++ "Perimeter = " ++ Z_to_string (perimeter_of_rectangle side1 side2))
+        (str ++ "Area = " ++ Z_to_string (area_of_rectangle side1 side2) ++ endl_content ++ "Perimeter = " ++ Z_to_string (perimeter_of_rectangle side1 side2))
   ).
 
   cpp.spec "areaRectangle(int, int)" from source inline.
